12/2/20 update

src/del/announcements.lean
@@ -1,7 +1,8 @@
 -- Following the textbook "Dynamic Epistemic Logic" by 
 -- Hans van Ditmarsch, Wiebe van der Hoek, and Barteld Kooi
 
-import del.languageDEL del.semantics.semanticsDEL data.set.basic
+import del.languageDEL del.semantics.semanticsDEL 
+import data.set.basic data.equiv.basic
 variable {agents : Type}
 local attribute [instance] classical.prop_decidable
 
@@ -42,32 +43,44 @@ split, intro h, intro h1, exact h1,
 rw forcesPA, trivial
 end
 
--- Proposition 4.12, pg. 77
-lemma public_announce_neg (φ ψ : formPA agents) : 
-  F_validPA (U φ (¬ψ) ↔ (φ ⊃ ¬(U φ ψ))) equiv_class :=
+--prop 4.22
+lemma public_annouce_var (φ : formPA agents) (f : frame agents) 
+  (v : nat → f.states → Prop) (x : f.states) (n : ℕ) :
+  forcesPA f v x (U φ p n) ↔ forcesPA f v x (φ ⊃ (p n)) :=
 begin
-rw F_validPA, intros f h1 v x, split,
+split, repeat {intros h1 h2, exact h1 h2},
+end
+
+lemma public_annouce_conj (φ ψ χ : formPA agents) (f : frame agents) 
+  (v : nat → f.states → Prop) (x : f.states) :
+  forcesPA f v x (U φ (ψ & χ)) ↔ forcesPA f v x ((U φ ψ) & (U φ χ)) :=
+begin
+split,
+intro h1,
+split,
+intro h2, specialize h1 h2,
+exact h1.left,
+intro h2, specialize h1 h2,
+exact h1.right, 
+intros h1 h2,
+split,
+exact h1.left h2,
+exact h1.right h2,
+end
+
+-- Proposition 4.12, pg. 77
+lemma public_announce_neg (φ ψ : formPA agents) (f : frame agents) 
+  (v : nat → f.states → Prop) (x : f.states) : 
+  forcesPA f v x (U φ (¬ψ)) ↔ forcesPA f v x (φ ⊃ ¬(U φ ψ))  :=
+begin
+split,
 intros h1 h2 h3, specialize h1 h2,
 specialize h3 h2, rw ←not_forces_impPA at h1,
 exact absurd h3 h1,
 intros h1, rw forcesPA at h1, rw imp_iff_not_or at h1,
 cases h1,
-intro h2, exact absurd h2 h1_1,
-intros h h1, apply h1_1, intro h2, exact h1
-end
-
--- Proposition 4.17, pg. 78
-lemma public_announce_comp (φ ψ χ : formPA agents) (f : frame agents) 
-  (v : nat → f.states → Prop) (s : f.states) :
-  forcesPA f v s (U (φ & U φ ψ) χ) ↔ forcesPA f v s (U φ (U ψ χ)) :=
-begin
-split,
-intro h1,
-intro h2, 
-sorry,
-intro h1,
-intro h2, 
-sorry
+intro h2, exact absurd h2 h1,
+intros h h2, apply h1, intro h3, exact h2
 end
 
 -- Proposition 4.18, pg. 79
@@ -91,27 +104,241 @@ intro hrel,
 exact h1 h2 t hrel h3,
 end
 
---prop 4.22
-lemma rwVar (φ : formPA agents) (f : frame agents) 
-  (v : nat → f.states → Prop) (x : f.states) (n : ℕ) :
-  forcesPA f v x (U φ p n) ↔ forcesPA f v x (φ ⊃ (p n)) :=
+namespace compositionPA
+
+-- -- The theory of x in m
+-- def theory_at (f : frame agents) (v : nat → f.states → Prop) (x : f.states) : 
+--   set (formPA agents) := { φ : formPA agents | forcesPA f v x φ}
+
+-- -- Invariance under bisimulation
+-- def base {f1 f2 : frame agents} (v1 : nat → f1.states → Prop) 
+--   (v2 : nat → f2.states → Prop) (x1 : f1.states) (x2 : f2.states) := 
+--   ∀ n, v1 n x1 ↔ v2 n x2
+
+-- def forth {f1 f2 : frame agents} (bisim : f1.states → f2.states → Prop) 
+--   (x1 : f1.states) (x2 : f2.states) := 
+--   ∀ a, ∀ y1, f1.rel a x1 y1 → (∃ y2 : f2.states, f2.rel a x2 y2 ∧ bisim y1 y2)
+
+-- def back {f1 f2 : frame agents} (bisim : f1.states → f2.states → Prop) 
+--   (x1 : f1.states) (x2 : f2.states) := 
+--   ∀ a, ∀ y2, f2.rel a x2 y2 → (∃ y1 : f1.states, f1.rel a x1 y1 ∧ bisim y1 y2)
+
+-- -- Bisimulation between M1 = (f1,v1) and M2 = (f2,v2)
+-- def is_bisimulation {f1 f2 : frame agents} (v1 : nat → f1.states → Prop) 
+--   (v2 : nat → f2.states → Prop) (bisim : f1.states → f2.states → Prop) := ∀ x1 x2,
+--   bisim x1 x2 → (base v1 v2 x1 x2 ∧ forth bisim x1 x2 ∧ back bisim x1 x2)
+
+-- theorem invariance_bisim {f1 f2 : frame agents} {v1 : nat → f1.states → Prop}
+--   {v2 : nat → f2.states → Prop} (bisim : f1.states → f2.states → Prop) 
+--   (h : is_bisimulation v1 v2 bisim) (x1 : f1.states) (x2 : f2.states) : 
+--   bisim x1 x2 → theory_at f1 v1 x1 = theory_at f2 v2 x2 :=
+-- begin
+-- intros h1, ext φ, revert x1 x2, induction φ,
+-- {intros x1 x2 h1, split, intro h2, exact h2, intro h2, exact h2}, 
+-- {intros x1 x2 h1, specialize h x1 x2 h1, cases h, 
+-- specialize h_left φ, cases h_left, split, intro h2, 
+-- exact h_left_mp h2, intro h2, exact h_left_mpr h2}, 
+-- {intros x1 x2 h1, specialize φ_ih_φ x1 x2 h1, specialize φ_ih_ψ x1 x2 h1, 
+-- cases φ_ih_φ, cases φ_ih_ψ, split, intro h2, cases h2, split, 
+-- exact φ_ih_φ_mp h2_left, exact φ_ih_ψ_mp h2_right, intro h2, 
+-- cases h2, split, exact φ_ih_φ_mpr h2_left, exact φ_ih_ψ_mpr h2_right}, 
+-- {intros x1 x2 h1, specialize φ_ih_φ x1 x2 h1, specialize φ_ih_ψ x1 x2 h1,
+-- cases φ_ih_φ, cases φ_ih_ψ, split, intros h2 h3, have h4 := φ_ih_φ_mpr h3,
+-- have h5 := h2 h4, exact φ_ih_ψ_mp h5, intros h2 h3, have h4 := φ_ih_φ_mp h3,
+-- have h5 := h2 h4, exact φ_ih_ψ_mpr h5},
+-- {rename φ_φ φ, intros x1 x2 h1, specialize h x1 x2 h1, cases h with h4 h5,
+-- cases h5 with h5 h6, split,
+-- {intros h2 y2 h3, specialize h6 φ_a y2 h3, cases h6 with y1 h6, 
+-- cases h6 with h6 h7, specialize h2 y1 h6, specialize φ_ih y1 y2 h7, 
+-- cases φ_ih, exact φ_ih_mp h2},
+-- {intros h2 y1 h3, specialize h5 φ_a y1 h3, cases h5 with y2 h5, 
+-- cases h5 with h5 h7, specialize h2 y2 h5, specialize φ_ih y1 y2 h7, 
+-- cases φ_ih, exact φ_ih_mpr h2}},
+-- {rename φ_φ φ, rename φ_ψ ψ, rename φ_ih_φ ih_φ, rename φ_ih_ψ ih_ψ,
+-- intros x1 x2 h1, specialize h x1 x2 h1, cases h with h2 h3,
+-- cases h3 with h3 h4, split,
+-- {
+--   intro h5,
+--   intro h6,
+--   rw theory_at at h5,
+--   rw set.mem_set_of_eq at h5,
+--   rw forcesPA at h5,
+--   specialize ih_φ x1 x2 h1,
+--   repeat {rw theory_at at ih_φ},
+--   repeat {rw set.mem_set_of_eq at ih_φ},
+--   have h7 := ih_φ.mpr h6,
+--   specialize h5 h7,
+--   specialize ih_ψ x1 x2 h1,
+--   repeat {rw theory_at at ih_ψ},
+--   repeat {rw set.mem_set_of_eq at ih_ψ},
+--   have h8 : forcesPA f1 v1 x1 ψ, 
+--   sorry,
+--   have h9 := ih_ψ.mp h8,
+--   sorry,
+-- }, 
+-- {
+--   intro h5,
+--   intro h6,
+--   rw theory_at at h5,
+--   rw set.mem_set_of_eq at h5,
+--   rw forcesPA at h5,
+--   specialize ih_φ x1 x2 h1,
+--   repeat {rw theory_at at ih_φ},
+--   repeat {rw set.mem_set_of_eq at ih_φ},
+--   have h7 := ih_φ.mp h6,
+--   specialize h5 h7,
+--   specialize ih_ψ x1 x2 h1,
+--   repeat {rw theory_at at ih_ψ},
+--   repeat {rw set.mem_set_of_eq at ih_ψ},
+--   have h8 : forcesPA f2 v2 x2 ψ, 
+--   sorry,
+--   have h9 := ih_ψ.mpr h8,
+--   sorry,
+-- }}
+-- end
+
+-- lemma comp_helper3 {f1 f2 : frame agents} {v1 : nat → f1.states → Prop} 
+--   {v2 : nat → f2.states → Prop} {x1 : f1.states} {x2 : f2.states} {φ : formPA agents} :
+--   forcesPA f1 v1 x1 φ → theory_at f1 v1 x1 = theory_at f2 v2 x2 → forcesPA f2 v2 x2 φ :=
+-- begin
+-- intros h1 h2,
+-- repeat {rw theory_at at h2},
+-- simp at *,
+-- repeat {rw set_of at h2},
+-- exact eq.subst h2 h1,
+-- end
+
+variables A A'     : Prop
+variable  B        : A → Prop
+variable  A''      : A' → Prop
+variable  B'       : ∀ h : A', A'' h → Prop
+
+lemma comp_helper1 (h : A ↔ ∃ h : A', A'' h) 
+  (h' : ∀ (h1 : A) (h2 : A') (h3 : A'' h2), B h1 ↔ B' h2 h3) : 
+  (∀ h1 : A, B h1) ↔ (∀ h2 h3, B' h2 h3) :=
 begin
-split, repeat {intros h1 h2, exact h1 h2},
+  split,
+  { intros hh h2 h3, 
+    have h1 : A := h.mpr ⟨h2, h3⟩,
+    exact (h' h1 h2 h3).mp (hh h1) },
+  intros hh h1,
+  cases h.mp h1 with h2 h3,
+  exact (h' h1 h2 h3).mpr (hh h2 h3)
 end
 
-lemma rwAnd (φ ψ χ : formPA agents) (f : frame agents) 
-  (v : nat → f.states → Prop) (x : f.states) (n : ℕ) :
-  forcesPA f v x (U φ (ψ & χ)) ↔ forcesPA f v x ((U φ ψ) & (U φ χ)) :=
+lemma comp_helper2 (φ ψ : formPA agents) (f : frame agents) 
+  (v : nat → f.states → Prop) (s : f.states) :
+  forcesPA f v s (φ & U φ ψ) ↔ 
+  (∃ h : forcesPA f v s φ, forcesPA (f.restrict 
+  (λ y, forcesPA f v y φ) s h) (λ n u, v n u.val) ⟨s, h⟩ ψ) :=
 begin
 split,
 intro h1,
+cases h1 with h1 h2,
+use h1, 
+apply h2,
+intro h1,
+cases h1 with h1 h2,
 split,
-intro h2, specialize h1 h2,
-exact h1.left,
-intro h2, specialize h1 h2,
-exact h1.right, 
-intros h1 h2,
-split,
-exact h1.left h2,
-exact h1.right h2,
+exact h1,
+intro h3,
+exact h2,
 end
+
+-- NEW LEMMAS START HERE --
+
+def is_modal_iso (f1 f2 : frame agents) (v1 : nat → f1.states → Prop)
+  (v2 : nat → f2.states → Prop) (F : f1.states ≃ f2.states) := 
+  ∀ x x' : f1.states, ∀ a : agents, (f1.rel a x x' ↔ f2.rel a (F x) (F x'))
+
+lemma update_iso {f1 f2 : frame agents} {v1 : nat → f1.states → Prop}
+  {v2 : nat → f2.states → Prop} (F : f1.states ≃ f2.states) :
+  is_modal_iso f1 f2 v1 v2 F → ∀ φ : formPA agents, ∀ x : f1.states,
+  ∀ h : forcesPA f1 v1 x φ, ∀ h' : forcesPA f2 v2 (F x) φ, 
+  ∃ F' : (f1.restrict (λ y, forcesPA f1 v1 y φ) x h).states
+  ≃ (f2.restrict (λ y, forcesPA f2 v2 y φ) (F x) h').states,
+  is_modal_iso (f1.restrict (λ y, forcesPA f1 v1 y φ) x h) 
+  (f2.restrict (λ y, forcesPA f2 v2 y φ) (F x) h') (λ n u, v1 n u.val) (λ n u, v2 n u.val) F' :=
+begin
+sorry
+end
+
+lemma comp_helper4 {f1 f2 : frame agents} {v1 : nat → f1.states → Prop} 
+  {v2 : nat → f2.states → Prop} (F : f1.states ≃ f2.states) :
+  (is_modal_iso f1 f2 v1 v2 F ∧ ∀ n : nat, ∀ x : f1.states, v1 n x = v2 n (F x)) → ∀ s1 : f1.states, 
+  ∀ φ : formPA agents, forcesPA f1 v1 s1 φ ↔ forcesPA f2 v2 (F s1) φ :=
+begin
+intro h1,
+cases h1 with h1 h2,
+intros x1 φ, induction φ generalizing x1,
+split,
+repeat {intro h3,
+exact h3},
+split,
+repeat {intro h3,
+rename φ n,
+specialize h2 n x1,
+rw forcesPA at *,
+convert h3},
+exact eq.symm h2,
+repeat {rename φ_φ φ}, 
+repeat {rename φ_ψ ψ},
+repeat {rename φ_ih_φ φ_ih},
+repeat {rename φ_ih_ψ ψ_ih},
+repeat {rename φ_a a},
+split,
+repeat {intro h3,
+rw forcesPA at *,
+cases h3 with h3 h4,
+split},
+exact (φ_ih x1).mp h3,
+exact (ψ_ih x1).mp h4,
+exact (φ_ih x1).mpr h3,
+exact (ψ_ih x1).mpr h4,
+split,
+repeat {intros h3 h4},
+exact (ψ_ih x1).mp (h3 ((φ_ih x1).mpr h4)),
+exact (ψ_ih x1).mpr (h3 ((φ_ih x1).mp h4)),
+split,
+intros h3 y1 h4,
+rw is_modal_iso at h1,
+specialize h3 (F.inv_fun y1),
+specialize φ_ih (F.inv_fun y1),
+specialize h1 x1 (F.inv_fun y1) a,
+simp at *,
+exact φ_ih.mp (h3 (h1.mpr h4)),
+intros h3 x2 h4,
+rw is_modal_iso at h1,
+specialize h1 x1 x2 a,
+specialize φ_ih x2,
+rw forcesPA at h3,
+specialize h3 (F.to_fun x2),
+simp at *,
+exact φ_ih.mpr (h3 (h1.mp h4)),
+split,
+intros h3 h4,
+specialize φ_ih x1,
+have h5 := update_iso F h1 φ x1 (φ_ih.mpr h4) h4,
+cases h5 with F' h5,
+rw forcesPA at h3,
+specialize h3 (φ_ih.mpr h4),
+repeat {sorry}
+end
+
+
+-- Proposition 4.17, pg. 78
+lemma public_announce_comp (φ ψ χ : formPA agents) (f : frame agents) 
+  (v : nat → f.states → Prop) (s : f.states) :
+  forcesPA f v s (U (φ & U φ ψ) χ) ↔ forcesPA f v s (U φ (U ψ χ)) :=
+begin
+apply comp_helper1,
+apply comp_helper2,
+intros h1 h2 h3,
+split,
+intro h4,
+--have h5 := comp_helper4,
+repeat {sorry}
+end
+
+end compositionPA
+
